proof tries before consolidating cvm_event and Ev datatypes

src/Axioms_Io.v
@@ -28,6 +28,20 @@ Admitted.
 Definition shuffled_events (el1:list Ev) (el2:list Ev) : list Ev.
 Admitted.
 
+Definition lts_remote_events (t:AnnoTerm) (p:Plc) : list Ev.
+Admitted.
+
+
+
+(*
+    Axiom remote_lts_axiom: forall a n et x,
+      lstar (conf a n et) x (stop n (aeval a n et)) ->
+      x = lts_remote_events a n.
+*)
+
+Axiom remote_LTS: forall t n et, 
+    lstar (conf t n et) (lts_remote_events t n) (stop n (aeval t n et)).
+
 
 
 Definition remote_evidence (t:AnnoTerm) (p:Plc) (e:EvC) : EvC.
@@ -50,6 +64,21 @@ Axiom at_events : forall t p,
 
 Axiom par_evidence : forall t (p:Plc) (e:EvC),
     parallel_vm_thread t p e = remote_evidence t p e.
+
+
+        Axiom par_events : forall t p,
+    parallel_vm_events t p = remote_trace t p.
+
+      Axiom bpar_shuffle : forall x tr p t1 t2 et1 et2,
+          lstar (conf t1 p et1) tr (stop p (aeval t1 p et1)) ->
+    lstar (bp x (conf t1 p et1) (conf t2 p et2))
+          (shuffled_events tr
+                           (lts_remote_events t2 p))
+          (bp x (stop p (aeval t1 p et1)) (stop p (aeval t2 p et2))).
+
+
+
+
 
 (*
 
